template-rocq/theories/Junk.v
@@ -1,0 +1,322 @@
+#[program]
+Definition of_level_map_n (m : LevelMap.t nat) V n (hne : ~ LevelMap.Empty m) : nonEmptyLevelExprSet :=
+  {| t_set := LevelMap.fold (fun l k acc =>
+    if LevelSet.mem l V then LevelExprSet.add (l, n + k) acc else
+    LevelExprSet.add (l, k) acc) m LevelExprSet.empty |}.
+Next Obligation. Admitted.
+
+Lemma of_level_map_n_spec m V hne :
+  forall l n k, LevelExprSet.In (l, k) (of_level_map_n m V n hne) ->
+    (exists k', LevelMap.MapsTo l k' m /\
+      (LevelSet.In l V -> k = n + k') /\
+      (~ LevelSet.In l V -> k = k')).
+Proof.
+Admitted.
+
+Lemma of_level_map_n_spec_inv m V hne :
+  forall l n k, LevelMap.MapsTo l k m ->
+    exists k', LevelExprSet.In (l, k') (of_level_map_n m V n hne) /\
+      (LevelSet.In l V -> k' = n + k) /\
+      (~ LevelSet.In l V -> k' = k).
+Proof.
+Admitted.
+
+
+Lemma of_level_map_of_level_map_n m V ne :
+  of_level_map m ne = of_level_map_n m V 0 ne.
+Proof.
+  apply eq_univ'.
+  intros [l k].
+  rewrite of_level_map_spec.
+  firstorder.
+  - unshelve eapply (of_level_map_n_spec_inv _ V ne _ 0) in H.
+    destruct H as [k' [hin [inv ninv]]].
+    destruct (inLevelSet V l) as [hvin|hnin].
+    specialize (inv hvin). cbn in inv. now subst k'.
+    specialize (ninv hnin). cbn in ninv. now subst.
+  - eapply of_level_map_n_spec in H as [k' [hm [hin hnin]]].
+    destruct (inLevelSet V l) as [hvin|hvnin].
+    now rewrite (hin hvin).
+    now rewrite (hnin hvnin).
+Qed.
+
+Lemma of_level_map_n_only_model m V n ne :
+
+  only_model_of V m ->
+  of_level_map_n m V n ne = add_prems n (of_level_map m ne).
+Proof.
+  intros om.
+  apply eq_univ'.
+  intros [l k].
+  rewrite In_add_prems.
+  split.
+  - move/of_level_map_n_spec => [k' [hm [hin hnin]]].
+    destruct (inLevelSet V l) as [hvin|hvnin].
+    * rewrite (hin hvin). exists (l, k').
+      rewrite of_level_map_spec. split => //. rewrite /add_expr. lia_f_equal.
+    * elim hvnin. apply om. now exists k'.
+  - intros [[? ?] [hin heq]]. unfold add_expr in heq; noconf heq.
+    unshelve eapply of_level_map_spec in hin.
+    have inv : LevelSet.In l V.
+    { apply om. now exists n0. }
+    eapply (of_level_map_n_spec_inv _ V ne _ n) in hin as [k' [hin [hinv hninv]]].
+    specialize (hinv inv). subst k'. now rewrite Nat.add_comm.
+Qed.
+
+
+(* Lemma entails_any V cls m nem m' nem' :
+  only_model_of V m ->
+  cls ⊢a of_level_map m nem → of_level_map m' nem' ->
+  model_rel_partial Nat.lt V m m' ->
+  cls ⊢a of_level_map m nem → of_level_map_n m V 1 nem.
+Proof.
+  intros tot cla mp [l k].
+  move/of_level_map_n_spec.
+  intros [k' [hm [hin hnin]]].
+  destruct (LevelSetDecide.MSetDecideAuxiliary.dec_In l V).
+  rewrite (hin H).
+  rewrite -[1 + _]Nat.add_1_r.
+  eapply entails_any_one; tea.
+  rewrite (hnin H).
+  constructor. now rewrite of_level_map_spec.
+Qed. *)
+
+(* Lemma entails_any V cls m nem m' nem' :
+  model_of V m ->
+  model_rel_partial Z.lt V m m' ->
+  cls ⊢a of_level_map_n m V 1 nem → of_level_map_n m V 2 nem.
+Proof. *)
+
+
+(* Lemma entails_concls cls V n m hne hne' :
+  model_of V m ->
+  entails_all cls (of_level_map_n m V n hne) (of_level_set V n hne').
+Proof.
+  move=> tot [l k].
+  rewrite levelexprset_of_levels_spec => [] [] hin ->.
+  specialize (tot _ hin) as [k' hm].
+  move/of_level_map_n_spec_inv in hm.
+  specialize (hm V hne n) as [k'' [hm [hin' hnin]]].
+  specialize (hin' hin). subst k''. cbn in *.
+  exists
+  depind ent.
+  - move: H.
+    rewrite of_level_map_n_spec => [] [k' [mt [hin hnin]]].
+    destruct (inLevelSet V l) as [H|H].
+    * now left.
+    * right. apply hnin in H. now subst k'.
+  - specialize (IHent _ _ _ en l).
+
+  intros [] *)
+
+(*
+Lemma strictly_updates_restrict cls V m m' :
+  strictly_updates cls V m m' ->
+  (forall cl, Clauses.In cl (cls_diff cls V) -> valid_clause m cl) ->
+  strictly_updates (cls ⇂ V) V m m'.
+Proof.
+  induction 1.
+  - intros hcl. constructor; auto.
+    move: {hcl} (hcl cl).
+    rewrite Clauses.diff_spec in_clauses_with_concl in_restrict_clauses.
+    destruct cl as [prems [concl k]]; cbn.
+    move=> h. split => //. eapply in_singleton.
+    forward h.
+    { split. split => //. apply in_singleton.
+    intros [insing hle incl'].
+    assert (~ LevelSet.Empty (levels prems)). admit.
+    have eqc : (forall l, LevelSet.In l (levels prems) -> l = concl).
+    { move=> l /hle. now rewrite LevelSet.singleton_spec. }
+    move: H0; rewrite /valid_clause //=.
+    intros [v [hmin hlt la eqm]].
+    destruct min_premise eqn:hm => //.
+    have [minple [minprem [inprems eqm]]] := min_premise_spec m prems.
+
+
+    assert (LevelSet.Equal (levels prems) (LevelSet.singleton concl)). split => //. lsets.
+    rewrite LevelSet.singleton_spec => ->. destruct (LevelSet.choose (levels prems)) eqn:hc.
+    apply LevelSet.choose_spec1 in hc. apply hle in hc. apply LevelSet.singleton_spec in hc; red in hc; subst.
+
+*)
+
+(*
+Lemma strictly_updates_entails_loop_relax cls V mzero hne m :
+  let bound := v_minus_w_bound V m in
+  let maxgain := max_gain cls in
+  let n := Z.to_nat bound + maxgain in
+  model_of V mzero ->
+  strictly_updates cls V mzero m ->
+  entails_all cls (of_level_map_n mzero V n hne) (of_level_map_n mzero V (n + 1) hne).
+Proof.
+  move=> bound maxgain n tot su.
+  have mp := strictly_updates_model_lt su tot.
+  have nem := strictly_updates_non_empty_map su.
+  eapply (strictly_updates_entails hne nem) in su; tea.
+  eapply entails_any in su; tea.
+  eapply (entails_all_shift n) in su.
+  rewrite -of_level_map_of_level_map_n.
+Qed.
+*)
+(* Lemma of_level_map_n_split m V n hne : of_level_map_n m V n hne = of_level_set V n hne'  *)
+Lemma max_premise_model_unique cls m : max_premise_model cls clauses_levels m -> m = max_premise_map cls.
+Proof.
+Admitted.
+
+
+(*
+Lemma strictly_updates_entails_loop_relax' ocls cls V (hne : ~ LevelSet.Empty V) mzero m :
+  above_max_premise_model ocls mzero ->
+  cls ⊂_clset ocls ->
+  V =_lset clauses_levels cls ->
+  model_of V mzero ->
+  strictly_updates cls V mzero m ->
+  entails_all cls (of_level_set V (max_clause_premise cls) hne)
+    (of_level_set V (max_clause_premise cls + 1) hne).
+Proof.
+  move=> habove hincl hv tot su.
+  eapply strictly_updates_entails_loop_relax; tea. *)
+
+
+
+(*
+Lemma above_max_premise_model_strengthen {cls cls' m} :
+  cls ⊂_clset cls' ->
+  above_max_premise_model cls m ->
+  above_max_premise_model cls' m.
+Proof.
+  intros hincl [[V' su]|eq].
+  left. 2:{ subst. red. } exists V'.
+  eapply strictly_updates_weaken; tea. red in ha.
+  move/(hmon _ _ hincl)/(ha l) => ha'.
+  eapply infer_atom_downward; tea.
+  apply max_clause_premise_mon in hincl. lia.
+Qed. *)
+Lemma model_max_max_premise_map cls : (model_max (max_premise_map cls)) = max_clause_premise cls.
+Proof.
+Admitted.
+
+
+
+Definition new_model m V newk : model :=
+  LevelMap.fold (fun l k acc =>
+    let k' := if LevelSet.mem l V then newk else k in
+    LevelMap.add l k' acc) m (LevelMap.empty _).
+
+Lemma new_model_spec m V newk l k :
+  LevelMap.MapsTo l k (new_model m V newk) ->
+  (exists k', LevelMap.MapsTo l k' m /\
+    if LevelSet.mem l V then k = newk else k = k').
+Proof. Admitted.
+
+Definition domain (l : LevelMap.t (option Z)) : LevelSet.t :=
+  LevelSetProp.of_list (List.map fst (LevelMap.elements l)).
+
+
+(* (forall cl', Clauses.In cl cls -> forall l k, LevelExprSet.In (l, k) (premise cl') -> k <= n) *)
+Lemma strictly_updates_entails_loop_max cls V (hne : ~ LevelSet.Empty V) m :
+  V =_lset clauses_levels cls ->
+  strictly_updates cls V (max_premise_map cls) m ->
+  entails_all cls (of_level_set V ((model_max (max_premise_map cls))) hne)
+    (of_level_set V ((model_max (max_premise_map cls)) + 1) hne).
+Proof.
+  intros.
+  rewrite !model_max_max_premise_map.
+  eapply strictly_updates_entails_loop; tea.
+  eapply max_premise_model_exists.
+  apply todo.
+Qed.
+
+
+Definition find_max (ls : LevelExprSet.t) (l : Level.t) :=
+  LevelExprSet.fold (fun '(l', k) acc => if eqb l l' then opt_max (Some k) acc else acc) ls None.
+
+Inductive find_max_spec ls l : option nat -> Prop :=
+| find_max_ex m : LevelExprSet.In (l, m) ls -> (forall k, LevelExprSet.In (l, k) ls -> k <= m) -> find_max_spec ls l (Some m)
+| find_max_absent : ~ (exists k, LevelExprSet.In (l, k) ls) -> find_max_spec ls l None.
+
+Lemma find_max_correct ls l : find_max_spec ls l (find_max ls l).
+Proof.
+  unfold find_max.
+  apply: (LevelExprSetProp.fold_rec (P := fun ls a => find_max_spec ls l a)).
+  - intros s' ise; constructor. intros [k hin]. now apply ise in hin.
+  - intros x a s' s'' hin hnotin hadd hspec.
+    destruct x as [l' k].
+    destruct (eqb_spec l l'); subst.
+    * depelim hspec.
+      { constructor. destruct (Nat.max_spec k m) as [[hle hm]|[hle hm]].
+        + rewrite hm. apply hadd; right; apply H.
+        + rewrite hm. apply hadd; left; reflexivity.
+        + intros k' hin'. apply hadd in hin' as [].
+          { noconf H1. lia. }
+          { specialize (H0 _ H1). lia. } }
+      { constructor. apply hadd; now left.
+        intros k0 hin'. apply hadd in hin' as [].
+        { noconf H0; reflexivity. }
+        { elim H. now exists k0. } }
+    * depelim hspec; constructor; eauto.
+      + apply hadd; now right.
+      + intros k' hin'. apply hadd in hin' as [].
+        { noconf H2. congruence. }
+        now apply H0 in H2.
+      + intros [k0 hk0]. apply hadd in hk0 as [].
+        { noconf H1; congruence. }
+        apply H. now exists k0.
+Qed.
+
+
+(* Lemma valuation_of_model_pos l k model : LevelMap.MapsTo l (Z.to_nat k) (valuation_of_model model) -> (k >= 0)%Z.
+Proof.
+  unfold valuation_of_model.
+  revert l k.
+  eapply LevelMapFact.fold_rec.
+  - intros. now rewrite LevelMapFact.F.empty_mapsto_iff in H0.
+  - intros l0 k0 e m' m'' me nk hadd hind l k.
+    rewrite LevelMapFact.F.add_mapsto_iff.
+    intros [].
+    * destruct H. red in H; subst.
+      destruct k0.
+      { have hmax := (model_max_spec model l (Some z) me). depelim hmax.
+        have hmin := (model_min_spec model l (Some z) me). depelim hmin.
+        assert (0 <= model_max model)%Z. admit.
+        assert (model_min model <= 0)%Z. admit.
+        assert (model_max model - option_get 0%Z (Some z) - model_min model = k)%Z. admit.
+        cbn in H4.
+        lia. *)
+
+
+
+
+Definition model_above cls m := forall l,
+  LevelSet.In l (clauses_levels cls) ->
+  exists k', LevelMap.MapsTo l k' m /\ max_clause_premise cls <= k'.
+
+Lemma model_above_infers {cls m} :
+  model_above cls m ->
+  (forall l, LevelSet.In l (clauses_levels cls) -> infers_atom m l (max_clause_premise cls)).
+Proof.
+Admitted.
+
+Lemma model_above_update {cls V' m m'} :
+  model_above cls m ->
+  strictly_updates cls V' m m' ->
+  model_above cls m'.
+Proof.
+  move=> above /strictly_updates_ext.
+  move=> le l /above => [] [] k' [] hm hle.
+  apply le in hm as [k'' [hin' le']].
+  exists k''. split => //. now transitivity k'.
+Qed.
+
+Lemma max_premise_model_above cls m : max_premise_model cls clauses_levels m -> model_above cls m.
+Admitted.
+
+
+(* Lemma max_premise_model_above cls sel sel' m :
+  (sel' cls ⊂_lset sel cls) ->
+  max_premise_model cls sel m ->
+  above_max_premise_model cls m.
+Proof.
+  move=> incl mp l hl; move: (proj1 mp l (incl _ hl)); rewrite /infers_atom.
+  move/level_value_MapsTo => ->. reflexivity.
+Qed. *)
+
